@prefix dc:    <http://purl.org/dc/elements/1.1/> .
@prefix app:   <http://jmvanel.free.fr/ontology/software_applications.owl#> .
@prefix list:  <http://www.w3.org/2000/10/swap/list#> .
@prefix log:   <http://www.w3.org/2000/10/swap/log#> .
@prefix grddl: <http://www.w3.org/2003/g/data-view#> .
@prefix rdfs:  <http://www.w3.org/2000/01/rdf-schema#> .
@prefix dbpedia: <http://dbpedia.org/resource/> .
@prefix dbo: <http://dbpedia.org/ontology/> .
@prefix owl:   <http://www.w3.org/2002/07/owl#> .
@prefix rdf:   <http://www.w3.org/1999/02/22-rdf-syntax-ns#> .
@prefix doap: <http://usefulinc.com/ns/doap#>.
@prefix foaf: <http://xmlns.com/foaf/0.1/> .
@prefix vann: <http://purl.org/vocab/vann/>.

@prefix doas:  <#> .

doas: a owl:Ontology ;
        rdfs:label "Description Of A Software" ;
        rdfs:comment  """Description Of A Software, a formal Description of a software focusing on architecture, feature, and input/output, enabling to search a software component according to needs,
and leveraging on dbPdedia.
complementary to DOAP."""@en ;
	foaf:maker <http://jmvanel.free.fr/jmv.rdf#me> ;
	vann:preferredNamespacePrefix "doas" ;
	foaf:homepage <http://deductions.github.io> .

doas:Software a       owl:Class ;
	rdfs:subclassOf doap:Project ;
        rdfs:label    "A software"@en ;
        rdfs:label    "Un logiciel"@fr ;
	owl:sameClassAs dbo:Software .
@base <https://deductions.github.io> .
doas:Software foaf:img <software.svg> .

doas:softwareType  a  owl:ObjectProperty ;
        rdfs:comment  "software type : client, server, library, compiler, etc (as dbPdedia URI)"@en ;
        rdfs:domain   doas:Software ;
        rdfs:label    "software type"@en ;
        rdfs:label    "type de logiciel"@fr .

doas:features  a      owl:ObjectProperty ;
        rdfs:comment  "features, as dbPdedia URI's"@en ;
        rdfs:domain   doas:Software ;
        rdfs:label    "features"@en ;
        rdfs:label    "fonctionnalités"@fr .

doas:outputFileTypes  a  owl:ObjectProperty ;
        rdfs:comment  "output file types, as dbPdedia URI's"@en ;
        rdfs:domain   doas:Software ;
        rdfs:label    "output file types"@en ;
        rdfs:label    "types de fichiers en sortie"@fr .

doas:inputFileTypes  a  owl:ObjectProperty ;
        rdfs:comment  "input file types, as dbPdedia URI's"@en ;
        rdfs:domain   doas:Software ;
        rdfs:label    "input file types"@en ;
        rdfs:label    "types de fichiers en entrée"@fr .

doas:uiTechnology  a  owl:ObjectProperty ;
        rdfs:comment  "User interface, a broad platform or library name, like web browser (dbpedia:HTML), Java Swing, TCL/TK, as dbPdedia URI's"@en ;
        rdfs:domain   doas:Software ;
        rdfs:label    "UI"@en ;
        rdfs:label    "IHM"@fr .

doas:dependencyManager a  owl:ObjectProperty ;
        rdfs:comment  "dependency Manager like npm, Maven, SBT, or explicitely dbpedia:Nothing, as dbPdedia URI's"@en ;
        rdfs:domain   doas:Software ;
        rdfs:label    "dependency Manager"@en ;
        rdfs:label    "Gestionnaire de dépendances"@fr .

dbo:programmingLanguage  a      owl:ObjectProperty ;
        rdfs:comment  "programming language, as dbPdedia URI's"@en ;
        rdfs:domain   doas:Software ;
        rdfs:label    "language (programming)"@en ;
        rdfs:label    "langage (de programmation)"@fr .

doas:modelingTechnology  a owl:ObjectProperty ;
        rdfs:comment  "modeling technology, as dbPdedia URI's; e.g. OWL, UML, SQL, Swagger, ..."@en ;
        rdfs:domain   doas:Software ;
        rdfs:label    "modeling technology"@en ;
        rdfs:label    "technologie de modélisation"@fr .

doas:isPluginOf a owl:ObjectProperty ;
        rdfs:comment  "embedding software if this sowftware is a plugin or module, as dbPdedia URI's; e.g. Firefox, Chrome, Apache, Protégé, ..."@en ;
        rdfs:domain   doas:Software ;
        rdfs:label    "plugin of"@en ;
        rdfs:label    "Additif dans (plugin)"@fr ;
        rdfs:range    doas:Software .

doas:hasDependency a owl:ObjectProperty ;
        rdfs:comment  "software (typically library) on which this sowftware depends; the plan is to get the information from a dependency Manager"@en ;
        rdfs:domain   doas:Software ;
        rdfs:label    "dependency"@en ;
        rdfs:label    "dépendance"@fr ;
        rdfs:range    doas:Software .

doas:powersWebSite a owl:ObjectProperty ;
        rdfs:domain   doas:Software ;
        rdfs:label    "a web site powered by this software"@en ;
        rdfs:label    "un site web propulsé par ce logiciel"@fr ;
        rdfs:comment  "for web service endpoint, use doap:service-endpoint"@en ;
        rdfs:range    foaf:Document .

doas:sandboxURL a owl:ObjectProperty ;
        rdfs:domain   doas:Software ;
        rdfs:label    "a sandbox web site powered by this software"@en ;
        rdfs:label    """un site web "bac à sable" propulsé par ce logiciel"""@fr ;
        rdfs:range    foaf:Document .

